\begin{appendices}

\section {Typing rules}

\subsection {System F}
\label{appendix:sysFrules}
\[\begin{array}{c@{\qquad}c}
    \mbox{\begin {prooftree}
      \hypo{x:\sigma \in \Gamma}
      \infer1[var]{\Gamma \vdash x:\sigma}
    \end {prooftree}}
    &
    \mbox{\begin{prooftree}
      \infer0[const]{\Gamma \vdash c:T}
    \end{prooftree}}
    \\\\
    \mbox{\begin{prooftree}
      \hypo{\Gamma, x:\sigma \vdash e : \tau}
      \infer1[abs]{\Gamma \vdash (\lambda x_\sigma \cdot e) : \sigma
        \to \tau}
    \end{prooftree}}
    &
    \mbox{\begin{prooftree}
      \hypo{\Gamma \vdash e_1 : \sigma \to \tau}
      \hypo{\Gamma \vdash e_2 : \sigma}
      \infer2[app]{\Gamma \vdash (e_1 e_2): \tau}
    \end{prooftree}}
    \\
\end{array} \]

Thus far the typing rules are the same as in the simply typed lambda
calculus, to complete his system Reynolds extends it with two more
rules to introduce parametric polymorphism:

\[\begin{array}{c@{\qquad}c}  
    \mbox{\begin{prooftree}
      \hypo{\Gamma \vdash M : \sigma}
      \infer1[$\Delta$-abs]{\Gamma \vdash (\Lambda \alpha \cdot M) : \Delta
      \alpha \cdot \sigma}
    \end{prooftree}}
    &
    \mbox{\begin{prooftree}
      \hypo{\Gamma \vdash M : \Delta \alpha \cdot \sigma}
      \infer1[$\Delta$-app]{\Gamma \vdash (M \tau) : \sigma[\tau / \alpha]}
    \end{prooftree}}
    \\\\
  \end{array} \]

Note that in these rules, $\alpha$ is a type variable.

\subsection {Hindley-Milner}
\label{appendix:HMrules}

In Hindley-Milner, we have very similar rules for typing lambda
abstraction, application, free type variables and and type constants:

\[\begin{array}{c@{\qquad}c}  
    \mbox{\begin{prooftree}
      \hypo{x : \sigma \in \Gamma}
      \infer1[var]{\Gamma \vdash x : \sigma}
    \end{prooftree}}
    &
    \mbox{\begin{prooftree}
      \infer0[const]{\Gamma \vdash c : T}
    \end{prooftree}}
    \\\\
    \mbox{\begin{prooftree}
      \hypo{\Gamma , x : \sigma \vdash e : \tau }
      \infer1[abs]{\Gamma \vdash (\lambda x \cdot e) : \sigma \to \tau}
    \end{prooftree}}
    &
    \mbox{\begin{prooftree}
      \hypo{\Gamma \vdash e_1 : \sigma \to \tau}
      \hypo{\Gamma \vdash e_2 : \sigma}
      \infer2[app]{\Gamma \vdash (e_1 e_2) : \tau}
    \end{prooftree}}
    \\\\      
\end{array} \]

These rules are then extended to accomodate the 'let' language
construct:

  \[\begin{array}{c}  
    \mbox{\begin{prooftree}
      \hypo{\Gamma \vdash e_1 : \sigma}
      \hypo{\Gamma, x : \sigma \vdash e_2 : \tau }
      \infer2[let]{\Gamma \vdash (let\; x = e_1\; in\; e_2) : \tau}
    \end{prooftree}}
    \\\\
  \end{array} \]

Before we detail the last two rules detailing instantiation and
generification we first outline the meaning of a judgement $\sigma
\sqsubseteq \sigma'$. Intuitively this means that $\sigma$ is some
subtype of $\sigma'$ - we can create it by some substitution of the
quantified variables in $\sigma'$. More precisely it is defined as
follows:

\[\begin{array}{c@{\qquad}c}  
    \mbox{\begin{prooftree}
      \hypo{\tau' = \{\alpha_i \mapsto \tau_i\}\tau}
      \hypo{\beta_i \notin free(\forall \alpha_1 \ldots \forall
        \alpha_n \cdot \tau)}
      \infer2[spec]{\forall \alpha_1 \ldots \forall \alpha_n \cdot
        \tau \sqsubseteq \forall \beta_1 \ldots \forall
        \beta_m \cdot \tau' }
    \end{prooftree}}
    \\\\
\end{array} \]  
  
Lastly we have rules to instantiate a type scheme, or generify a
type (i.e. to make a type more specific and narrow, or less specific
and general):

\[\begin{array}{c@{\qquad}c}  
    \mbox{\begin{prooftree}
      \hypo{\Gamma \vdash e : \sigma}
      \hypo{\sigma' \sqsubseteq \sigma}
      \infer2[inst]{\Gamma \vdash e : \sigma'}
    \end{prooftree}}
    &
    \mbox{\begin{prooftree}
      \hypo{\Gamma \vdash e : \sigma}
      \hypo{\alpha \notin free(\Gamma)}
      \infer2[gen]{\Gamma \vdash e : \forall \alpha \sigma}
    \end{prooftree}}
    \\\\
\end{array} \]

The latter three rules are the ones that capture the idea of
Hindley-Milner polymorphism.

\clearpage
\section{Example specifications}
\label{appendix:examplespecifications}

This appendix shows example specification files for various
languages.

\subsection{Simply typed lambda calculus with product types}
\label{STLCspec}

\begin{verbatim}
type: α
  value: a

type: β
  value: b

type: A -> B
  if:
    type A
    type B
  eliminated-by: E
    if:
      (A) <- E
    resulting-in-type: B
  value: \ X. -> M
    if:
      X : (A) |- (B) <- M
    reduces-to: M/[, E:A]
  expanded-by: \ Y. -> Y
  
type: A x B
  if:
    type A
    type B
  eliminated-by: fst
    resulting-in-type: A
  eliminated-by: snd
    resulting-in-type: B
  value: L and R
    if:
      (A) <- L
      (B) <- R
    reduces-to: L
    reduces-to: R
  expanded-by: fst , snd
\end{verbatim}

\clearpage
\subsection{System-F-like language}
\label{SystemFspec}

Our variation is slighly more general than the original encoding as
opposed to only polymorphic functions we give the means of
representing arbitrary polymorphic types.

\begin{verbatim}
type: α
  value: a

type: β
  value: b

type: A -> B
  if:
    type A
    type B
  eliminated-by: E
    if:
      (A) <- E
    resulting-in-type: B
  value: \ X. -> M
    if:
      X : (A) |- (B) <- M
    reduces-to: M/[, E:A]
  expanded-by: \ Y. -> Y

type: ∀ T. => M
  if:
    T : (set) |- type M
  eliminated-by: TY
    if:
      type TY
    resulting-in-type: M/[, TY:set]
  value: δ T. PTY
    if:
      T : (set) |- (M/[, .T]) <- PTY
    reduces-to: PTY/[, TY:set]
\end{verbatim}

\clearpage
\subsection{Lambda calculus variation with dependent types}
\label{DTLCspec}

\begin{verbatim}
type: α
  value: a1
  value: a2

type: isa TY TM
  if:
    type TY
    (TY) <- TM
  value: is V
    if:
      (TY) <- V
      (TM) = V

type: A X. -> B
  if:
    type A
    X : (A) |- type B
  eliminated-by: E
    if:
      (A) <- E
    resulting-in-type: B/[, E:A]
  value: \ X. -> M
    if:
      X : (A) |- (B/[, .X]) <- M
    reduces-to: M/[, E:A]
  expanded-by: \ Y. -> Y
\end{verbatim}
\clearpage
\section{Parser combinators}
\label{appendix-parsercombinators}

\begin{verbatim}
fail : Parser A
fail str = nothing

-- guarantees a parser, if it succeeds, consumes some input
safe : Parser A → Parser A
safe p s = do
             (a , leftover) ← p s
             if length leftover <ᵇ length s then just (a , leftover) else nothing
           where open maybemonad

peak : Parser Char
peak str with toList str
... | []      = nothing
... | c ∷ rest = just ((c , fromList (c ∷ rest)))

all : Parser String
all = λ s → just (s , "")

try : Parser A → A → Parser A
try p a str = p str <∣> just (a , str)

consumes : Parser A → Parser (ℕ × A)
consumes p = do
               bfr ← (λ s → just (length s , s))
               a ← p
               afr ← (λ s → just (length s , s))
               return (∣ bfr - afr ∣ , a)
             where open parsermonad

biggest-of_and_ : Parser A → Parser A → Parser A
biggest-of_and_ p1 p2 str with p1 str | p2 str
... | nothing | nothing = nothing
... | nothing | just p = just p
... | just p | nothing = just p
... | just (a1 , rst1) | just (a2 , rst2) = just (if length rst1 <ᵇ length rst2 then (a1 , rst1) else (a2 , rst2))

_or_ : Parser A → Parser B → Parser (A ⊎ B)
(pa or pb) str = (inj₁ <$> pa) str <∣> (inj₂ <$> pb) str
  where
    open parsermonad

either_or_ : Parser A → Parser A → Parser A
(either pa or pb) str = maybe′ just (pb str) (pa str)

ifp_then_else_ : Parser A → Parser B → Parser B → Parser B
(ifp p then pthen else pelse) str with p str
... | nothing = pelse str
... | just x  = pthen str

nout : Parser ⊤
nout = return tt
  where open parsermonad

optional : Parser A → Parser (A ⊎ ⊤)
optional = _or nout

complete : Parser A → Parser A
complete p = do
               a ← p
               rest ← all
               if rest ==ˢ "" then return a else fail
             where open parsermonad

takeIfc : (Char → Bool) → Parserp Char
takeIfc p []          = nothing
takeIfc p (c ∷ chars) = if p c then just (c , chars) else nothing

takeIf : (Char → Bool) → Parser Char
takeIf p = →[ takeIfc p ]→

-- This terminates as we ensure to make p "safe" before we
-- use it, forcing the parser to fail if it does not consume
-- any input
{-# TERMINATING #-}
_*[_,_] : Parser A → (A → B → B) → B → Parser B
p *[ f , b ] = do
                 inj₁ a ← optional (safe p)
                   where inj₂ _ → return b
                 b ← p *[ f , b ] 
                 return (f a b)
  where open parsermonad


_⁺[_,_] : Parser A → (A → B → B) → B → Parser B
p ⁺[ f , b ] = pure f ⊛ p ⊛ (p *[ f , b ])
  where open parsermonad

anyof : List (Parser A) → Parser A
anyof []       = fail
anyof (p ∷ ps) = either p or (anyof ps)

biggest-consumer : List (Parser A) → Parser A
biggest-consumer [] = fail
biggest-consumer (p ∷ ps) = biggest-of p and biggest-consumer ps

all-of : List (Parser A) → Parser (List A)
all-of [] str = just ([] , str)
all-of ps str = just (foldr (λ p las → maybe′ (λ (a , _) → a ∷ las) las (p str) ) [] ps , "")

{-# TERMINATING #-}
how-many? : Parser A → Parser (Σ[ n ∈ ℕ ] Vec A n)
how-many? p = ifp p then (do
                            a ←  safe p
                            (n , as) ← how-many? p
                            return (ℕ.suc n , a ∷ as))
              else return (0 , [])
  where open parsermonad

max_how-many? : ℕ → Parser A → Parser (Σ[ n ∈ ℕ ] Vec A n)
max zero how-many? _    = return (0 , [])
  where open parsermonad
max (suc n) how-many? p = ifp p then (do
                            a ←  safe p
                            (n , as) ← max n how-many? p
                            return (ℕ.suc n , a ∷ as))
              else return (0 , [])
  where open parsermonad

exactly : (n : ℕ) → Parser A → Parser (Vec A n)
exactly zero _  = return []
  where open parsermonad
exactly (suc n) p = do
                      a ← p
                      as ← exactly n p
                      return (a ∷ as)
-- text/number parsing

whitespace : Parser ⊤
whitespace str = just (tt , trim← str)

ws+nl : Parser ⊤
ws+nl str = just (tt , trim←p str)

ws+nl! : Parser ⊤
ws+nl! = do
            c ← takeIf Data.Char.isSpace
            ws+nl
           where open parsermonad

ws-tolerant : Parser A → Parser A
ws-tolerant p = do
                  whitespace
                  r ← p
                  whitespace
                  return r
  where open parsermonad

wsnl-tolerant : Parser A → Parser A
wsnl-tolerant p = do
                    ws+nl
                    r ← p
                    ws+nl
                    return r
  where open parsermonad

wsnl-tolerant! : Parser A → Parser A
wsnl-tolerant! p = do
                    ws+nl!
                    r ← p
                    ws+nl!
                    return r
  where open parsermonad

literalc : Char → Parserp Char
literalc c [] = nothing
literalc c (x ∷ rest)
  = if c == x then just (c , rest)
              else nothing

literal : Char → Parser Char
literal c = →[ literalc c ]→

newline = literal "\n"

nextCharc : Parserp Char
nextCharc []          = nothing
nextCharc (c ∷ chars) = just (c , chars)

nextChar = →[ nextCharc ]→

literalAsString = (fromChar <$>_) ∘′ literal
  where open parsermonad

string : String → Parser String
string str = foldr
                 (λ c p → (pure _++_) ⊛ (literalAsString c) ⊛ p)
                 (return "") (toList str)
  where open parsermonad

  
stringof : (Char → Bool) → Parser String
stringof p = takeIf p *[ _++_ ∘ fromChar , "" ]

until : (Char → Bool) → Parser String
until p = stringof (not ∘ p)

nonempty : Parser String → Parser String
nonempty p = do
               r ← p
               if r ==ˢ "" then (λ _ → nothing) else return r
  where open parsermonad

nat : Parser ℕ
nat = do
        d ← nonempty (stringof isDigit)
        return (toNat d)
      where open parsermonad


bracketed : Parser A → Parser A
bracketed p = do
                literal "("
                a ← wsnl-tolerant p
                literal ")"
                return a
   where open parsermonad

potentially-bracketed : Parser A → Parser A
potentially-bracketed p = either bracketed p or p

curlybracketed : Parser A → Parser A
curlybracketed p = do
                literal "{"
                a ← wsnl-tolerant p
                literal "}"
                return a
  where open parsermonad

squarebracketed : Parser A → Parser A
squarebracketed p = do
                literal "["
                a ← wsnl-tolerant p
                literal "]"
                return a
  where open parsermonad
  open Parsers
\end{verbatim}

\section{A selection of testing code}
\label{appendix-tests}

\subsection{Description of STLC}
\input{../../src/latex/Test/Specs/STLC.tex}

\subsection{Beta reduction and normalisation}
\input{../../src/latex/Test/BetaTest.tex}

\subsection{Eta expansion}
\input{../../src/latex/Test/EtaTest.tex}

\subsection{Type checking STLC}
\input{../../src/latex/Test/STLCTest.tex}
\clearpage
\section{Lattice meet/join algorithms}
\label{appendix-joinalgorithms}

We simplify these algorithms by ignoring scope, in practice we would
need to consider scope if we were to use these algorithms in our code.

The following algorithm may be used to calculate the join of a set
of patterns.

\begin{enumerate}
\item Consider all the topmost data constructors in the patterns
  (disregarding places).
  \begin{enumerate}
  \item if they are not all the same then the join is a \emph{place}
  \item if they are all \emph{atoms}
    \begin{enumerate}
    \item if they are all the same atom, then the join is that atom
      \item if they are all different atoms, then the join is a \emph{place}
    \end{enumerate}
  \item if they were all \emph{place}s then the join is a \emph{place}
  \item if the are all \emph{⊥}s then the join is \emph{⊥}  
  \item if they are all pairs
    \begin{enumerate}
      \item calculate the join of all the left elements $J_l$
      \item calulate the join of all the right elements $J_r$
      \item the join is the pair ($J_l$ ∙ $J_r$)
    \end{enumerate}
  \item if they are all binds
    \begin{enumerate}
    \item calculate the join of the terms under all the binders $J_b$
    \item the join is (bind $J_b$)
    \end{enumerate}
  \end{enumerate}
\end{enumerate}

The following algorithm may be used to calculate the meet of a set
of patterns.

\begin{enumerate}
\item Consider all the topmost data constructors in the patterns
  (disregarding places).
  \begin{enumerate}
  \item if they are not all the same then the meet is \emph{⊥}
  \item if they are all \emph{atoms}
    \begin{enumerate}
    \item if they are all the same atom, then the meet is that atom.
      \item if they are all different atoms, then the meet is \emph{⊥}
    \end{enumerate}
  \item if they were all \emph{place}s then the meet is a \emph{place}
  \item if the are all \emph{⊥}s then the meet is \emph{⊥}  
  \item if they are all pairs
    \begin{enumerate}
      \item calculate the meet of all the left elements $M_l$
      \item calulate the meet of all the right elements $M_r$
      \item the meet is the pair ($M_l$ ∙ $M_r$)
    \end{enumerate}
  \item if they are all binds
    \begin{enumerate}
    \item calculate the meet of the terms under all the binders $M_b$
    \item the meet is (bind $M_b$)
    \end{enumerate}
  \end{enumerate}
\end{enumerate}

\end{appendices}
